<?xml version="1.0"?>
<rdf:RDF xmlns="https://raw.githubusercontent.com/lucvaladares/GeoCoreOntology/master/GeoCoreOntology.owl"
     xml:base="https://raw.githubusercontent.com/lucvaladares/GeoCoreOntology/master/GeoCoreOntology.owl"
     xmlns:dc="http://purl.org/dc/elements/1.1/"
     xmlns:obo="http://purl.obolibrary.org/obo/"
     xmlns:owl="http://www.w3.org/2002/07/owl#"
     xmlns:rdf="http://www.w3.org/1999/02/22-rdf-syntax-ns#"
     xmlns:xml="http://www.w3.org/XML/1998/namespace"
     xmlns:xsd="http://www.w3.org/2001/XMLSchema#"
     xmlns:foaf="http://xmlns.com/foaf/0.1/"
     xmlns:rdfs="http://www.w3.org/2000/01/rdf-schema#"
     xmlns:skos="http://www.w3.org/2004/02/skos/core#"
     xmlns:GeoCoreOntology="https://raw.githubusercontent.com/lucvaladares/GeoCoreOntology/master/GeoCoreOntology.owl#">
    <owl:Ontology rdf:about="https://raw.githubusercontent.com/lucvaladares/GeoCoreOntology/master/GeoCoreOntology.owl">
        <owl:imports rdf:resource="http://purl.obolibrary.org/obo/bfo/iso/2020/bfo.owl"/>
        <dc:contributor>Luan Fonseca Garcia</dc:contributor>
        <dc:contributor xml:lang="en">Mara Abel</dc:contributor>
        <dc:contributor xml:lang="en">Michel Perrin</dc:contributor>
    </owl:Ontology>
    


    <!-- 
    ///////////////////////////////////////////////////////////////////////////////////////
    //
    // Annotation properties
    //
    ///////////////////////////////////////////////////////////////////////////////////////
     -->

    


    <!-- http://purl.obolibrary.org/obo/IAO_0000112 -->

    <owl:AnnotationProperty rdf:about="http://purl.obolibrary.org/obo/IAO_0000112"/>
    


    <!-- http://purl.obolibrary.org/obo/IAO_0000115 -->

    <owl:AnnotationProperty rdf:about="http://purl.obolibrary.org/obo/IAO_0000115"/>
    


    <!-- http://purl.obolibrary.org/obo/IAO_0000116 -->

    <owl:AnnotationProperty rdf:about="http://purl.obolibrary.org/obo/IAO_0000116"/>
    


    <!-- http://purl.obolibrary.org/obo/IAO_0000119 -->

    <owl:AnnotationProperty rdf:about="http://purl.obolibrary.org/obo/IAO_0000119"/>
    


    <!-- 
    ///////////////////////////////////////////////////////////////////////////////////////
    //
    // Object Properties
    //
    ///////////////////////////////////////////////////////////////////////////////////////
     -->

    


    <!-- https://raw.githubusercontent.com/lucvaladares/GeoCoreOntology/master/GeoCoreOntology.owl#UFRGS_GCO_age_of -->

    <owl:ObjectProperty rdf:about="https://raw.githubusercontent.com/lucvaladares/GeoCoreOntology/master/GeoCoreOntology.owl#UFRGS_GCO_age_of">
        <rdfs:subPropertyOf rdf:resource="http://purl.obolibrary.org/obo/BFO_0000197"/>
        <owl:inverseOf rdf:resource="https://raw.githubusercontent.com/lucvaladares/GeoCoreOntology/master/GeoCoreOntology.owl#UFRGS_GCO_has_age"/>
        <obo:IAO_0000115 xml:lang="en">The relation between a Geological Age and a Geological Object. Inverse of has age relation.</obo:IAO_0000115>
        <rdfs:label xml:lang="en">age of</rdfs:label>
    </owl:ObjectProperty>
    


    <!-- https://raw.githubusercontent.com/lucvaladares/GeoCoreOntology/master/GeoCoreOntology.owl#UFRGS_GCO_carrier_of -->

    <owl:ObjectProperty rdf:about="https://raw.githubusercontent.com/lucvaladares/GeoCoreOntology/master/GeoCoreOntology.owl#UFRGS_GCO_carrier_of">
        <rdfs:subPropertyOf rdf:resource="http://www.w3.org/2002/07/owl#topObjectProperty"/>
        <rdfs:domain rdf:resource="http://purl.obolibrary.org/obo/BFO_0000004"/>
        <rdfs:range rdf:resource="http://purl.obolibrary.org/obo/BFO_0000031"/>
        <obo:IAO_0000112 xml:lang="en">Molecules of DNA are carriers of genetic information</obo:IAO_0000112>
        <obo:IAO_0000112 xml:lang="en">This copy of War and Peace is carrier of the novel written by Tolstoy</obo:IAO_0000112>
        <obo:IAO_0000112 xml:lang="en">This hard drive is carrier of these data items</obo:IAO_0000112>
        <obo:IAO_0000115 xml:lang="en">The relation between an independent continuant that is not a spatial region and is the carrier of some g-dependent continuant</obo:IAO_0000115>
        <obo:IAO_0000116 xml:lang="en">This relation was defined in the BFO 2020 text. We added it in the GeoCore Ontology because the RO ontology didn&apos;t add it yet.</obo:IAO_0000116>
        <obo:IAO_0000119 xml:lang="en">BFO 2020</obo:IAO_0000119>
        <rdfs:label>carrier of</rdfs:label>
    </owl:ObjectProperty>
    


    <!-- https://raw.githubusercontent.com/lucvaladares/GeoCoreOntology/master/GeoCoreOntology.owl#UFRGS_GCO_constituted_by -->

    <owl:ObjectProperty rdf:about="https://raw.githubusercontent.com/lucvaladares/GeoCoreOntology/master/GeoCoreOntology.owl#UFRGS_GCO_constituted_by">
        <rdfs:subPropertyOf rdf:resource="http://www.w3.org/2002/07/owl#topObjectProperty"/>
        <rdf:type rdf:resource="http://www.w3.org/2002/07/owl#AsymmetricProperty"/>
        <rdf:type rdf:resource="http://www.w3.org/2002/07/owl#IrreflexiveProperty"/>
        <obo:IAO_0000115>The relation between some material entity and the material that it is made of.</obo:IAO_0000115>
        <obo:IAO_0000119>Evnine, S. J. (2011). Constitution and composition: Three approaches to their relation. ProtoSociology, 27, 212-235.</obo:IAO_0000119>
        <rdfs:label xml:lang="en">constituted by</rdfs:label>
    </owl:ObjectProperty>
    


    <!-- https://raw.githubusercontent.com/lucvaladares/GeoCoreOntology/master/GeoCoreOntology.owl#UFRGS_GCO_filled -->

    <owl:ObjectProperty rdf:about="https://raw.githubusercontent.com/lucvaladares/GeoCoreOntology/master/GeoCoreOntology.owl#UFRGS_GCO_filled">
        <rdfs:subPropertyOf rdf:resource="http://purl.obolibrary.org/obo/BFO_0000171"/>
        <rdfs:domain rdf:resource="http://purl.obolibrary.org/obo/BFO_0000040"/>
        <rdfs:range rdf:resource="http://purl.obolibrary.org/obo/BFO_0000029"/>
        <rdfs:label xml:lang="en">filled</rdfs:label>
    </owl:ObjectProperty>
    


    <!-- https://raw.githubusercontent.com/lucvaladares/GeoCoreOntology/master/GeoCoreOntology.owl#UFRGS_GCO_filled_by -->

    <owl:ObjectProperty rdf:about="https://raw.githubusercontent.com/lucvaladares/GeoCoreOntology/master/GeoCoreOntology.owl#UFRGS_GCO_filled_by">
        <rdfs:subPropertyOf rdf:resource="http://purl.obolibrary.org/obo/BFO_0000124"/>
        <rdfs:label xml:lang="en">filled by</rdfs:label>
    </owl:ObjectProperty>
    


    <!-- https://raw.githubusercontent.com/lucvaladares/GeoCoreOntology/master/GeoCoreOntology.owl#UFRGS_GCO_generated_by -->

    <owl:ObjectProperty rdf:about="https://raw.githubusercontent.com/lucvaladares/GeoCoreOntology/master/GeoCoreOntology.owl#UFRGS_GCO_generated_by">
        <rdfs:subPropertyOf rdf:resource="http://purl.obolibrary.org/obo/BFO_0000056"/>
        <rdf:type rdf:resource="http://www.w3.org/2002/07/owl#AsymmetricProperty"/>
        <rdf:type rdf:resource="http://www.w3.org/2002/07/owl#IrreflexiveProperty"/>
        <obo:IAO_0000115>A relation between a continuant and a process, in which the continuant was generated by the process</obo:IAO_0000115>
        <rdfs:label xml:lang="en">generated by</rdfs:label>
    </owl:ObjectProperty>
    


    <!-- https://raw.githubusercontent.com/lucvaladares/GeoCoreOntology/master/GeoCoreOntology.owl#UFRGS_GCO_generated_in -->

    <owl:ObjectProperty rdf:about="https://raw.githubusercontent.com/lucvaladares/GeoCoreOntology/master/GeoCoreOntology.owl#UFRGS_GCO_generated_in">
        <rdfs:subPropertyOf rdf:resource="http://www.w3.org/2002/07/owl#topObjectProperty"/>
        <obo:IAO_0000115 xml:lang="en">The Geological Time Interval in which the object was generated.</obo:IAO_0000115>
        <rdfs:label xml:lang="en">generated in</rdfs:label>
    </owl:ObjectProperty>
    


    <!-- https://raw.githubusercontent.com/lucvaladares/GeoCoreOntology/master/GeoCoreOntology.owl#UFRGS_GCO_genetic_role_of -->

    <owl:ObjectProperty rdf:about="https://raw.githubusercontent.com/lucvaladares/GeoCoreOntology/master/GeoCoreOntology.owl#UFRGS_GCO_genetic_role_of">
        <rdfs:subPropertyOf rdf:resource="http://purl.obolibrary.org/obo/BFO_0000197"/>
        <owl:inverseOf rdf:resource="https://raw.githubusercontent.com/lucvaladares/GeoCoreOntology/master/GeoCoreOntology.owl#UFRGS_GCO_has_genetic_role"/>
        <rdfs:label xml:lang="en">genetic role of</rdfs:label>
    </owl:ObjectProperty>
    


    <!-- https://raw.githubusercontent.com/lucvaladares/GeoCoreOntology/master/GeoCoreOntology.owl#UFRGS_GCO_has_age -->

    <owl:ObjectProperty rdf:about="https://raw.githubusercontent.com/lucvaladares/GeoCoreOntology/master/GeoCoreOntology.owl#UFRGS_GCO_has_age">
        <rdfs:subPropertyOf rdf:resource="http://purl.obolibrary.org/obo/BFO_0000196"/>
        <obo:IAO_0000115 xml:lang="en">The relation between a Geological Object and its Geological Age.</obo:IAO_0000115>
        <rdfs:label xml:lang="en">has age</rdfs:label>
    </owl:ObjectProperty>
    


    <!-- https://raw.githubusercontent.com/lucvaladares/GeoCoreOntology/master/GeoCoreOntology.owl#UFRGS_GCO_has_genetic_role -->

    <owl:ObjectProperty rdf:about="https://raw.githubusercontent.com/lucvaladares/GeoCoreOntology/master/GeoCoreOntology.owl#UFRGS_GCO_has_genetic_role">
        <rdfs:subPropertyOf rdf:resource="http://purl.obolibrary.org/obo/BFO_0000196"/>
        <rdfs:domain rdf:resource="http://purl.obolibrary.org/obo/BFO_0000040"/>
        <rdfs:range rdf:resource="https://raw.githubusercontent.com/lucvaladares/GeoCoreOntology/master/GeoCoreOntology.owl#UFRGS_GCO_genetic_role"/>
        <rdfs:label>has genetic role</rdfs:label>
    </owl:ObjectProperty>
    


    <!-- 
    ///////////////////////////////////////////////////////////////////////////////////////
    //
    // Classes
    //
    ///////////////////////////////////////////////////////////////////////////////////////
     -->

    


    <!-- https://raw.githubusercontent.com/lucvaladares/GeoCoreOntology/master/GeoCoreOntology.owl#UFRGS_GCO_earth_fluid -->

    <owl:Class rdf:about="https://raw.githubusercontent.com/lucvaladares/GeoCoreOntology/master/GeoCoreOntology.owl#UFRGS_GCO_earth_fluid">
        <rdfs:subClassOf rdf:resource="https://raw.githubusercontent.com/lucvaladares/GeoCoreOntology/master/GeoCoreOntology.owl#UFRGS_GCO_earth_material"/>
        <owl:disjointWith rdf:resource="https://raw.githubusercontent.com/lucvaladares/GeoCoreOntology/master/GeoCoreOntology.owl#UFRGS_GCO_rock"/>
        <obo:IAO_0000115 xml:lang="en">Earth fluid is an &apos;earth material&apos; that is fluild.

They can be water, oil, gas or a mixture of those fluids.</obo:IAO_0000115>
        <rdfs:label xml:lang="en">earth fluid</rdfs:label>
        <rdfs:label xml:lang="pt">fluido da terra</rdfs:label>
    </owl:Class>
    


    <!-- https://raw.githubusercontent.com/lucvaladares/GeoCoreOntology/master/GeoCoreOntology.owl#UFRGS_GCO_earth_material -->

    <owl:Class rdf:about="https://raw.githubusercontent.com/lucvaladares/GeoCoreOntology/master/GeoCoreOntology.owl#UFRGS_GCO_earth_material">
        <rdfs:subClassOf rdf:resource="http://purl.obolibrary.org/obo/BFO_0000040"/>
        <obo:IAO_0000115 xml:lang="en">Earth material is a &apos;material entity&apos; that is a natural amount of matter, which is solid, fluid or unconsolidated. Earth materials are generated by some &apos;geological process&apos;.

They are rigid entities with a definite identity criteria, but no unifying relation.</obo:IAO_0000115>
        <rdfs:label xml:lang="en">earth material</rdfs:label>
        <rdfs:label xml:lang="pt">material geologico</rdfs:label>
    </owl:Class>
    


    <!-- https://raw.githubusercontent.com/lucvaladares/GeoCoreOntology/master/GeoCoreOntology.owl#UFRGS_GCO_genetic_role -->

    <owl:Class rdf:about="https://raw.githubusercontent.com/lucvaladares/GeoCoreOntology/master/GeoCoreOntology.owl#UFRGS_GCO_genetic_role">
        <rdfs:subClassOf rdf:resource="http://purl.obolibrary.org/obo/BFO_0000023"/>
        <rdfs:subClassOf>
            <owl:Restriction>
                <owl:onProperty rdf:resource="http://purl.obolibrary.org/obo/BFO_0000054"/>
                <owl:qualifiedCardinality rdf:datatype="http://www.w3.org/2001/XMLSchema#nonNegativeInteger">1</owl:qualifiedCardinality>
                <owl:onClass rdf:resource="https://raw.githubusercontent.com/lucvaladares/GeoCoreOntology/master/GeoCoreOntology.owl#UFRGS_GCO_geological_process"/>
            </owl:Restriction>
        </rdfs:subClassOf>
        <rdfs:label xml:lang="en">genetic role</rdfs:label>
    </owl:Class>
    


    <!-- https://raw.githubusercontent.com/lucvaladares/GeoCoreOntology/master/GeoCoreOntology.owl#UFRGS_GCO_geological_age -->

    <owl:Class rdf:about="https://raw.githubusercontent.com/lucvaladares/GeoCoreOntology/master/GeoCoreOntology.owl#UFRGS_GCO_geological_age">
        <rdfs:subClassOf rdf:resource="http://purl.obolibrary.org/obo/BFO_0000019"/>
        <obo:IAO_0000115 xml:lang="en">It is a Quality of Geological Object related to a Geological Time Interval during which some Geological Process operated. The age of a Geological Object is the age of the process that generated this object.</obo:IAO_0000115>
        <rdfs:label xml:lang="en">geological age</rdfs:label>
        <rdfs:label xml:lang="pt">idade geológica</rdfs:label>
    </owl:Class>
    


    <!-- https://raw.githubusercontent.com/lucvaladares/GeoCoreOntology/master/GeoCoreOntology.owl#UFRGS_GCO_geological_boundary -->

    <owl:Class rdf:about="https://raw.githubusercontent.com/lucvaladares/GeoCoreOntology/master/GeoCoreOntology.owl#UFRGS_GCO_geological_boundary">
        <rdfs:subClassOf rdf:resource="http://purl.obolibrary.org/obo/BFO_0000140"/>
        <obo:IAO_0000115 xml:lang="en">A Geological Boundary is a Continuant Fiat Boundary corresponding to a physical discontinuity of any nature, located on the external surface of a Geological Object.</obo:IAO_0000115>
        <rdfs:label xml:lang="en">geological boundary</rdfs:label>
        <rdfs:label xml:lang="pt">limite geológico</rdfs:label>
    </owl:Class>
    


    <!-- https://raw.githubusercontent.com/lucvaladares/GeoCoreOntology/master/GeoCoreOntology.owl#UFRGS_GCO_geological_contact -->

    <owl:Class rdf:about="https://raw.githubusercontent.com/lucvaladares/GeoCoreOntology/master/GeoCoreOntology.owl#UFRGS_GCO_geological_contact">
        <rdfs:subClassOf rdf:resource="http://purl.obolibrary.org/obo/BFO_0000145"/>
        <obo:IAO_0000115 xml:lang="en">It is a Relational Quality which relates two Geologic Objects having the same dimension (1D, 2D, or 3D), whose external boundaries are adjacent to each other.</obo:IAO_0000115>
        <rdfs:label xml:lang="pt">contato geológico</rdfs:label>
        <rdfs:label xml:lang="en">geological contact</rdfs:label>
    </owl:Class>
    


    <!-- https://raw.githubusercontent.com/lucvaladares/GeoCoreOntology/master/GeoCoreOntology.owl#UFRGS_GCO_geological_object -->

    <owl:Class rdf:about="https://raw.githubusercontent.com/lucvaladares/GeoCoreOntology/master/GeoCoreOntology.owl#UFRGS_GCO_geological_object">
        <owl:equivalentClass>
            <owl:Class>
                <owl:intersectionOf rdf:parseType="Collection">
                    <rdf:Description rdf:about="http://purl.obolibrary.org/obo/BFO_0000030"/>
                    <owl:Restriction>
                        <owl:onProperty rdf:resource="https://raw.githubusercontent.com/lucvaladares/GeoCoreOntology/master/GeoCoreOntology.owl#UFRGS_GCO_has_age"/>
                        <owl:someValuesFrom rdf:resource="https://raw.githubusercontent.com/lucvaladares/GeoCoreOntology/master/GeoCoreOntology.owl#UFRGS_GCO_geological_age"/>
                    </owl:Restriction>
                    <owl:Restriction>
                        <owl:onProperty rdf:resource="https://raw.githubusercontent.com/lucvaladares/GeoCoreOntology/master/GeoCoreOntology.owl#UFRGS_GCO_constituted_by"/>
                        <owl:allValuesFrom rdf:resource="https://raw.githubusercontent.com/lucvaladares/GeoCoreOntology/master/GeoCoreOntology.owl#UFRGS_GCO_earth_material"/>
                    </owl:Restriction>
                    <owl:Restriction>
                        <owl:onProperty rdf:resource="https://raw.githubusercontent.com/lucvaladares/GeoCoreOntology/master/GeoCoreOntology.owl#UFRGS_GCO_generated_by"/>
                        <owl:allValuesFrom rdf:resource="https://raw.githubusercontent.com/lucvaladares/GeoCoreOntology/master/GeoCoreOntology.owl#UFRGS_GCO_geological_process"/>
                    </owl:Restriction>
                    <owl:Restriction>
                        <owl:onProperty rdf:resource="https://raw.githubusercontent.com/lucvaladares/GeoCoreOntology/master/GeoCoreOntology.owl#UFRGS_GCO_has_genetic_role"/>
                        <owl:allValuesFrom rdf:resource="https://raw.githubusercontent.com/lucvaladares/GeoCoreOntology/master/GeoCoreOntology.owl#UFRGS_GCO_genetic_role"/>
                    </owl:Restriction>
                </owl:intersectionOf>
            </owl:Class>
        </owl:equivalentClass>
        <owl:equivalentClass>
            <owl:Restriction>
                <owl:onProperty rdf:resource="https://raw.githubusercontent.com/lucvaladares/GeoCoreOntology/master/GeoCoreOntology.owl#UFRGS_GCO_genetic_role_of"/>
                <owl:someValuesFrom rdf:resource="https://raw.githubusercontent.com/lucvaladares/GeoCoreOntology/master/GeoCoreOntology.owl#UFRGS_GCO_geological_object"/>
            </owl:Restriction>
        </owl:equivalentClass>
        <obo:IAO_0000115 xml:lang="en">A Geological Object is a rigid entity that provides its own identity and holds a unity criteria. A Geological Object is constituted by Earth Material and is generated by some Geological Process.</obo:IAO_0000115>
        <rdfs:label xml:lang="en">geological object</rdfs:label>
        <rdfs:label xml:lang="pt">objeto geológico</rdfs:label>
    </owl:Class>
    


    <!-- https://raw.githubusercontent.com/lucvaladares/GeoCoreOntology/master/GeoCoreOntology.owl#UFRGS_GCO_geological_process -->

    <owl:Class rdf:about="https://raw.githubusercontent.com/lucvaladares/GeoCoreOntology/master/GeoCoreOntology.owl#UFRGS_GCO_geological_process">
        <rdfs:subClassOf rdf:resource="http://purl.obolibrary.org/obo/BFO_0000015"/>
        <rdfs:subClassOf>
            <owl:Restriction>
                <owl:onProperty rdf:resource="http://purl.obolibrary.org/obo/BFO_0000055"/>
                <owl:someValuesFrom rdf:resource="https://raw.githubusercontent.com/lucvaladares/GeoCoreOntology/master/GeoCoreOntology.owl#UFRGS_GCO_genetic_role"/>
            </owl:Restriction>
        </rdfs:subClassOf>
        <obo:IAO_0000115 xml:lang="en">It is a physical, chemical or biological process or series of processes that generate, destroy or modify the shape, the internal arrangement or the composition of at least one Geological Object.</obo:IAO_0000115>
        <rdfs:label xml:lang="en">geological process</rdfs:label>
        <rdfs:label xml:lang="pt">processo geológico</rdfs:label>
    </owl:Class>
    


    <!-- https://raw.githubusercontent.com/lucvaladares/GeoCoreOntology/master/GeoCoreOntology.owl#UFRGS_GCO_geological_structure -->

    <owl:Class rdf:about="https://raw.githubusercontent.com/lucvaladares/GeoCoreOntology/master/GeoCoreOntology.owl#UFRGS_GCO_geological_structure">
        <rdfs:subClassOf rdf:resource="http://purl.obolibrary.org/obo/BFO_0000031"/>
        <obo:IAO_0000115 xml:lang="en">It is a Generically Dependent Continuant which describes the internal arrangement of a Geological Object, i.e., the configuration and the mutual relationships of its different parts.</obo:IAO_0000115>
        <rdfs:label xml:lang="pt">estrutura geológica</rdfs:label>
        <rdfs:label xml:lang="en">geological structure</rdfs:label>
    </owl:Class>
    


    <!-- https://raw.githubusercontent.com/lucvaladares/GeoCoreOntology/master/GeoCoreOntology.owl#UFRGS_GCO_geological_time_interval -->

    <owl:Class rdf:about="https://raw.githubusercontent.com/lucvaladares/GeoCoreOntology/master/GeoCoreOntology.owl#UFRGS_GCO_geological_time_interval">
        <rdfs:subClassOf rdf:resource="http://purl.obolibrary.org/obo/BFO_0000038"/>
        <obo:IAO_0000115 xml:lang="en">It is a Temporal Region of one dimension within the Global Geological Time. A Geological Time Interval may be occupied by one or several Geological Processes.</obo:IAO_0000115>
        <rdfs:label xml:lang="en">geological time interval</rdfs:label>
        <rdfs:label xml:lang="pt">intervalo de tempo geológico</rdfs:label>
    </owl:Class>
    


    <!-- https://raw.githubusercontent.com/lucvaladares/GeoCoreOntology/master/GeoCoreOntology.owl#UFRGS_GCO_mineral -->

    <owl:Class rdf:about="https://raw.githubusercontent.com/lucvaladares/GeoCoreOntology/master/GeoCoreOntology.owl#UFRGS_GCO_mineral">
        <rdfs:subClassOf rdf:resource="https://raw.githubusercontent.com/lucvaladares/GeoCoreOntology/master/GeoCoreOntology.owl#UFRGS_GCO_earth_material"/>
        <obo:IAO_0000115 xml:lang="en">Mineral is an &apos;earth material&apos; that is an inorganic, solid, and homogenous chemical compound with crystalline structure.</obo:IAO_0000115>
        <rdfs:label xml:lang="en">mineral</rdfs:label>
        <rdfs:label xml:lang="pt">mineral</rdfs:label>
    </owl:Class>
    


    <!-- https://raw.githubusercontent.com/lucvaladares/GeoCoreOntology/master/GeoCoreOntology.owl#UFRGS_GCO_rock -->

    <owl:Class rdf:about="https://raw.githubusercontent.com/lucvaladares/GeoCoreOntology/master/GeoCoreOntology.owl#UFRGS_GCO_rock">
        <rdfs:subClassOf rdf:resource="https://raw.githubusercontent.com/lucvaladares/GeoCoreOntology/master/GeoCoreOntology.owl#UFRGS_GCO_earth_material"/>
        <obo:IAO_0000115 xml:lang="en">Rock is a solid consolidated &apos;earth material&apos; that is made of mineral matter, or material of mineral origin.</obo:IAO_0000115>
        <obo:IAO_0000116 xml:lang="en">Geologists define rock at a scale of observation where they consider it a homogeneous mass.</obo:IAO_0000116>
        <rdfs:label xml:lang="pt">rocha</rdfs:label>
        <rdfs:label xml:lang="en">rock</rdfs:label>
    </owl:Class>
    


    <!-- https://raw.githubusercontent.com/lucvaladares/GeoCoreOntology/master/GeoCoreOntology.owl#UFRGS_GCO_site_location_role -->

    <owl:Class rdf:about="https://raw.githubusercontent.com/lucvaladares/GeoCoreOntology/master/GeoCoreOntology.owl#UFRGS_GCO_site_location_role">
        <rdfs:subClassOf rdf:resource="http://purl.obolibrary.org/obo/BFO_0000023"/>
        <rdfs:label xml:lang="en">site location role</rdfs:label>
    </owl:Class>
    


    <!-- https://raw.githubusercontent.com/lucvaladares/GeoCoreOntology/master/GeoCoreOntology.owl#UFRGS_GCO_unconsolidated_earth_material -->

    <owl:Class rdf:about="https://raw.githubusercontent.com/lucvaladares/GeoCoreOntology/master/GeoCoreOntology.owl#UFRGS_GCO_unconsolidated_earth_material">
        <rdfs:subClassOf rdf:resource="https://raw.githubusercontent.com/lucvaladares/GeoCoreOntology/master/GeoCoreOntology.owl#UFRGS_GCO_earth_material"/>
        <obo:IAO_0000115 xml:lang="en">Unconsolidated earth material is an &apos;earth material&apos; that is consituted by an aggregate of solid particles but is not consolidated into a &apos;rock&apos; it self.</obo:IAO_0000115>
        <rdfs:label xml:lang="pt">material geológico inconsolidado</rdfs:label>
        <rdfs:label xml:lang="en">unconsolidated earth material</rdfs:label>
    </owl:Class>
    


    <!-- 
    ///////////////////////////////////////////////////////////////////////////////////////
    //
    // Individuals
    //
    ///////////////////////////////////////////////////////////////////////////////////////
     -->

    


    <!-- https://raw.githubusercontent.com/lucvaladares/GeoCoreOntology/master/GeoCoreOntology.owl#go_1 -->

    <owl:NamedIndividual rdf:about="https://raw.githubusercontent.com/lucvaladares/GeoCoreOntology/master/GeoCoreOntology.owl#go_1">
        <GeoCoreOntology:UFRGS_GCO_generated_by rdf:resource="https://raw.githubusercontent.com/lucvaladares/GeoCoreOntology/master/GeoCoreOntology.owl#gp_1"/>
        <GeoCoreOntology:UFRGS_GCO_has_genetic_role rdf:resource="https://raw.githubusercontent.com/lucvaladares/GeoCoreOntology/master/GeoCoreOntology.owl#role_1"/>
    </owl:NamedIndividual>
    


    <!-- https://raw.githubusercontent.com/lucvaladares/GeoCoreOntology/master/GeoCoreOntology.owl#gp_1 -->

    <owl:NamedIndividual rdf:about="https://raw.githubusercontent.com/lucvaladares/GeoCoreOntology/master/GeoCoreOntology.owl#gp_1"/>
    


    <!-- https://raw.githubusercontent.com/lucvaladares/GeoCoreOntology/master/GeoCoreOntology.owl#role_1 -->

    <owl:NamedIndividual rdf:about="https://raw.githubusercontent.com/lucvaladares/GeoCoreOntology/master/GeoCoreOntology.owl#role_1">
        <rdf:type rdf:resource="https://raw.githubusercontent.com/lucvaladares/GeoCoreOntology/master/GeoCoreOntology.owl#UFRGS_GCO_genetic_role"/>
    </owl:NamedIndividual>
    


    <!-- 
    ///////////////////////////////////////////////////////////////////////////////////////
    //
    // General axioms
    //
    ///////////////////////////////////////////////////////////////////////////////////////
     -->

    <rdf:Description>
        <rdf:type rdf:resource="http://www.w3.org/2002/07/owl#AllDisjointClasses"/>
        <owl:members rdf:parseType="Collection">
            <rdf:Description rdf:about="http://purl.obolibrary.org/obo/BFO_0000024"/>
            <rdf:Description rdf:about="http://purl.obolibrary.org/obo/BFO_0000027"/>
            <rdf:Description rdf:about="http://purl.obolibrary.org/obo/BFO_0000030"/>
            <rdf:Description rdf:about="https://raw.githubusercontent.com/lucvaladares/GeoCoreOntology/master/GeoCoreOntology.owl#UFRGS_GCO_earth_material"/>
        </owl:members>
    </rdf:Description>
    <rdf:Description>
        <rdf:type rdf:resource="http://www.w3.org/2002/07/owl#AllDisjointClasses"/>
        <owl:members rdf:parseType="Collection">
            <rdf:Description rdf:about="https://raw.githubusercontent.com/lucvaladares/GeoCoreOntology/master/GeoCoreOntology.owl#UFRGS_GCO_earth_fluid"/>
            <rdf:Description rdf:about="https://raw.githubusercontent.com/lucvaladares/GeoCoreOntology/master/GeoCoreOntology.owl#UFRGS_GCO_mineral"/>
            <rdf:Description rdf:about="https://raw.githubusercontent.com/lucvaladares/GeoCoreOntology/master/GeoCoreOntology.owl#UFRGS_GCO_rock"/>
        </owl:members>
    </rdf:Description>
    <rdf:Description>
        <rdf:type rdf:resource="http://www.w3.org/2002/07/owl#AllDisjointClasses"/>
        <owl:members rdf:parseType="Collection">
            <rdf:Description rdf:about="https://raw.githubusercontent.com/lucvaladares/GeoCoreOntology/master/GeoCoreOntology.owl#UFRGS_GCO_earth_fluid"/>
            <rdf:Description rdf:about="https://raw.githubusercontent.com/lucvaladares/GeoCoreOntology/master/GeoCoreOntology.owl#UFRGS_GCO_mineral"/>
            <rdf:Description rdf:about="https://raw.githubusercontent.com/lucvaladares/GeoCoreOntology/master/GeoCoreOntology.owl#UFRGS_GCO_rock"/>
            <rdf:Description rdf:about="https://raw.githubusercontent.com/lucvaladares/GeoCoreOntology/master/GeoCoreOntology.owl#UFRGS_GCO_unconsolidated_earth_material"/>
        </owl:members>
    </rdf:Description>
</rdf:RDF>



<!-- Generated by the OWL API (version 4.5.9.2019-02-01T07:24:44Z) https://github.com/owlcs/owlapi -->

